Hacl.Operations: make sure not to use the 'pos' ML-reserved keyword

crypto_hst/utils/Hacl.Operations.fst
@@ -122,15 +122,15 @@ let rec nor_bytes output in1 len =
 // Setall
 //
 
-val setall': (b:bytes) -> (l:u32{length b = v l}) -> (x:s8) -> (pos:u32{v pos <= length b /\ v pos < pow2 32})
+val setall': (b:bytes) -> (l:u32{length b = v l}) -> (x:s8) -> (posi:u32{v posi <= length b /\ v posi < pow2 32})
   -> STL unit
         (requires (fun h -> live h b))
         (ensures  (fun h0 _ h1 -> live h1 b /\ modifies_1 b h0 h1))
 
-let rec setall' buf buflen x pos =
-  if lt pos buflen then begin
-    SB.upd buf pos x;
-    setall' buf buflen x (U32.add pos 1ul)  end
+let rec setall' buf buflen x posi =
+  if lt posi buflen then begin
+    SB.upd buf posi x;
+    setall' buf buflen x (U32.add posi 1ul)  end
   else ()
 
 
@@ -157,55 +157,55 @@ let setmask1 b l v = setall' b l v 0ul
 // Setmask2
 //
 
-val setmask2': mask:bytes -> masklen:u32{v masklen = SB.length mask /\ v masklen < pow2 32} -> byteval1:s8 -> byteval2:s8 -> pos:s32{v pos <= v masklen} -> i:u32{v i >= 0 /\ v i <= v masklen}
+val setmask2': mask:bytes -> masklen:u32{v masklen = SB.length mask /\ v masklen < pow2 32} -> byteval1:s8 -> byteval2:s8 -> posi:s32{v posi <= v masklen} -> i:u32{v i >= 0 /\ v i <= v masklen}
   -> STL unit
         (requires (fun h -> live h mask))
         (ensures  (fun h0 _ h1 -> live h1 mask /\ modifies_1 mask h0 h1))
 
-let rec setmask2' mask masklen b1 b2 pos i =
+let rec setmask2' mask masklen b1 b2 posi i =
   if U32.lt i masklen then
-    let m32 = S32.lt_mask (uint32_to_sint32 i) pos in
+    let m32 = S32.lt_mask (uint32_to_sint32 i) posi in
     let m8 = sint32_to_sint8 m32 in
     let b = S8.logor (S8.logand m8 b1)
                      (S8.logand (S8.lognot m8) b2) in
     SB.upd mask i b;
-    setmask2' mask masklen b1 b2 pos (U32.add i 1ul)
+    setmask2' mask masklen b1 b2 posi (U32.add i 1ul)
   else ()
 
-val setmask2: mask:bytes -> masklen:u32{v masklen = SB.length mask /\ v masklen < pow2 32} -> byteval1:s8 -> byteval2:s8 -> pos:s32{v pos <= v masklen}
+val setmask2: mask:bytes -> masklen:u32{v masklen = SB.length mask /\ v masklen < pow2 32} -> byteval1:s8 -> byteval2:s8 -> posi:s32{v posi <= v masklen}
   -> STL unit
         (requires (fun h -> live h mask))
         (ensures  (fun h0 _ h1 -> live h1 mask /\ modifies_1 mask h0 h1))
-let setmask2 mask masklen b1 b2 pos = setmask2' mask masklen b1 b2 pos 0ul
+let setmask2 mask masklen b1 b2 posi = setmask2' mask masklen b1 b2 posi 0ul
 
 
 //
 // Setmask3
 //
 
-val setmask3': mask:bytes -> masklen:u32{v masklen = SB.length mask /\ v masklen < pow2 32} -> byteval1:s8 -> byteval2:s8 -> byteval3:s8 -> pos1:s32{v pos1 <= v masklen} -> pos2:s32{v pos1 < v pos2 /\ v pos2 <= v masklen} -> i:u32{v i >= 0 /\ v i <= v masklen}
+val setmask3': mask:bytes -> masklen:u32{v masklen = SB.length mask /\ v masklen < pow2 32} -> byteval1:s8 -> byteval2:s8 -> byteval3:s8 -> posi1:s32{v posi1 <= v masklen} -> posi2:s32{v posi1 < v posi2 /\ v posi2 <= v masklen} -> i:u32{v i >= 0 /\ v i <= v masklen}
   -> STL unit
         (requires (fun h -> live h mask))
         (ensures  (fun h0 _ h1 -> live h1 mask /\ modifies_1 mask h0 h1))
 
-let rec setmask3' mask masklen b1 b2 b3 pos1 pos2 i =
+let rec setmask3' mask masklen b1 b2 b3 posi1 posi2 i =
   if U32.lt i masklen then
-    let c1  = sint32_to_sint8 (S32.gte_mask (uint32_to_sint32 i) pos1) in
-    let c2  = sint32_to_sint8 (S32.gte_mask (uint32_to_sint32 i) pos2) in
+    let c1  = sint32_to_sint8 (S32.gte_mask (uint32_to_sint32 i) posi1) in
+    let c2  = sint32_to_sint8 (S32.gte_mask (uint32_to_sint32 i) posi2) in
     let nc2 = S8.lognot c2 in
     let r1 = S8.logand b1 (S8.logand (S8.lognot c1) (S8.lognot c2)) in
     let r2 = S8.logand b2 (S8.logand c1 (S8.lognot c2)) in
     let r3 = S8.logand b3 (S8.logand c1 c2) in
     let b = S8.logor r1 (S8.logor r2 r3) in
     SB.upd mask i b;
-    setmask3' mask masklen b1 b2 b3 pos1 pos2 (U32.add i 1ul)
+    setmask3' mask masklen b1 b2 b3 posi1 posi2 (U32.add i 1ul)
   else ()
 
-val setmask3: mask:bytes -> masklen:u32{v masklen = SB.length mask /\ v masklen < pow2 32} -> byteval1:s8 -> byteval2:s8 -> byteval3:s8 -> pos1:s32{v pos1 <= v masklen} -> pos2:s32{v pos1 < v pos2 /\ v pos2 <= v masklen}
+val setmask3: mask:bytes -> masklen:u32{v masklen = SB.length mask /\ v masklen < pow2 32} -> byteval1:s8 -> byteval2:s8 -> byteval3:s8 -> posi1:s32{v posi1 <= v masklen} -> posi2:s32{v posi1 < v posi2 /\ v posi2 <= v masklen}
   -> STL unit
         (requires (fun h -> live h mask))
         (ensures  (fun h0 _ h1 -> live h1 mask /\ modifies_1 mask h0 h1))
-let setmask3 mask masklen b1 b2 b3 pos1 pos2 = setmask3' mask masklen b1 b2 b3 pos1 pos2 0ul
+let setmask3 mask masklen b1 b2 b3 posi1 posi2 = setmask3' mask masklen b1 b2 b3 posi1 posi2 0ul
 
 
 //
